src/Stc/StcTyping.v
@@ -39,36 +39,36 @@ Module Type STCTYPING
        (Import Syn   : STCSYNTAX Ids Op CESyn)
        (Import CETyp : CETYPING  Ids Op CESyn).
 
-  Inductive wt_trconstr (P: program) (vars: list (ident * type)) (lasts: list (ident * type)): trconstr -> Prop :=
+  Inductive wt_trconstr (P: program) (vars: list (ident * type)) (inits: list (ident * type)): trconstr -> Prop :=
   | wt_TcDef:
       forall x ck e,
         In (x, typeofc e) vars ->
-        wt_clock (vars ++ lasts) ck ->
-        wt_cexp (vars ++ lasts) e ->
-        wt_trconstr P vars lasts (TcDef x ck e)
+        wt_clock (vars ++ inits) ck ->
+        wt_cexp (vars ++ inits) e ->
+        wt_trconstr P vars inits (TcDef x ck e)
   | wt_TcNext:
       forall x ck e,
-        In (x, typeof e) lasts ->
-        wt_clock (vars ++ lasts) ck ->
-        wt_exp (vars ++ lasts) e ->
-        wt_trconstr P vars lasts (TcNext x ck e)
+        In (x, typeof e) inits ->
+        wt_clock (vars ++ inits) ck ->
+        wt_exp (vars ++ inits) e ->
+        wt_trconstr P vars inits (TcNext x ck e)
   | wt_TcReset:
       forall s ck f i P',
         find_system f P = Some (s, P') ->
-        wt_clock (vars ++ lasts) ck ->
-        wt_trconstr P vars lasts (TcReset i ck f)
+        wt_clock (vars ++ inits) ck ->
+        wt_trconstr P vars inits (TcReset i ck f)
   | wt_TcCall:
       forall s xs ck rst f es i P',
         find_system f P = Some (s, P') ->
         Forall2 (fun x '(_, (t, _)) => In (x, t) vars) xs s.(s_out) ->
         Forall2 (fun e '(_, (t, _)) => typeof e = t) es s.(s_in) ->
-        wt_clock (vars ++ lasts) ck ->
-        Forall (wt_exp (vars ++ lasts)) es ->
-        wt_trconstr P vars lasts (TcCall i xs ck rst f es).
+        wt_clock (vars ++ inits) ck ->
+        Forall (wt_exp (vars ++ inits)) es ->
+        wt_trconstr P vars inits (TcCall i xs ck rst f es).
 
   Definition wt_system (P: program) (s: system) : Prop :=
     Forall (wt_trconstr P (idty (s.(s_in) ++ s.(s_vars) ++ s.(s_out)))
-                        (map (fun x => (fst x, type_const (fst (snd x)))) s.(s_lasts)))
+                        (map (fun x => (fst x, type_const (fst (snd x)))) s.(s_inits)))
            s.(s_tcs).
 
   (* TODO: replace Welldef_global; except for the Is_well_sch component.
@@ -93,14 +93,14 @@ Module Type STCTYPING
                 ==> @eq trconstr ==> iff)
            wt_trconstr.
   Proof.
-    intros G1 G2 HG env1 env2 Henv lasts1 lasts2 Hlasts eq1 eq2 Heq.
+    intros G1 G2 HG env1 env2 Henv inits1 inits2 Hinits eq1 eq2 Heq.
     subst.
     split; intro WTtc.
-    - inv WTtc; rewrite Henv, Hlasts in *; econstructor; eauto;
+    - inv WTtc; rewrite Henv, Hinits in *; econstructor; eauto;
         match goal with H:Forall2 _ ?x ?y |- Forall2 _ ?x ?y =>
                         apply Forall2_impl_In with (2:=H) end;
         intros ? (?&(?&?)); rewrite Henv in *; auto.
-    - inv WTtc; rewrite <-Henv, <-Hlasts in *; econstructor; eauto;
+    - inv WTtc; rewrite <-Henv, <-Hinits in *; econstructor; eauto;
           match goal with H:Forall2 _ ?x ?y |- Forall2 _ ?x ?y =>
                           apply Forall2_impl_In with (2:=H) end;
           intros ? (?&(?&?)); rewrite Henv in *; auto.
