src/Instantiator.v
@@ -54,7 +54,7 @@ From Velus Require Import StcToObc.Stc2ObcInvariants.
 From Velus Require Import StcToObc.Stc2ObcTyping.
 
 Module Stc2Obc     := TranslationFun     Ids Op OpAux CE.Syn Stc.Syn Obc.Syn.
-Module MemCorres   := StcMemoryCorresFun Ids Op       CE.Syn Stc.Syn Stc.Last.
+Module MemCorres   := StcMemoryCorresFun Ids Op       CE.Syn Stc.Syn Stc.Init.
 Module Stc2ObcCorr := CorrectnessFun     Ids Op OpAux IStr CE Stc Obc Stc2Obc MemCorres.
 
 Module Stc2ObcInvariants := Stc2ObcInvariantsFun Ids Op OpAux IStr CE Stc Obc Stc2Obc.
