src/Stc/Stc.v
@@ -16,7 +16,7 @@ From Velus Require Export Stc.StcSyntax.
 From Velus Require Export Stc.StcIsSystem.
 From Velus Require Export Stc.StcOrdered.
 From Velus Require Export Stc.StcSemantics.
-From Velus Require Export Stc.StcIsLast.
+From Velus Require Export Stc.StcIsInit.
 From Velus Require Export Stc.StcIsVariable.
 From Velus Require Export Stc.StcIsDefined.
 From Velus Require Export Stc.StcIsFree.
@@ -40,19 +40,19 @@ Module Type STC
   Declare Module Export Syst : STCISSYSTEM    Ids Op       CE.Syn Syn.
   Declare Module Export Ord  : STCORDERED     Ids Op       CE.Syn Syn Syst.
   Declare Module Export Sem  : STCSEMANTICS   Ids Op OpAux CE.Syn Syn Syst Ord Str CE.Sem.
-  Declare Module Export Last : STCISLAST      Ids Op       CE.Syn Syn.
+  Declare Module Export Init : STCISINIT      Ids Op       CE.Syn Syn.
   Declare Module Export Var  : STCISVARIABLE  Ids Op       CE.Syn Syn.
-  Declare Module Export Def  : STCISDEFINED   Ids Op       CE.Syn Syn Var Last.
+  Declare Module Export Def  : STCISDEFINED   Ids Op       CE.Syn Syn Var Init.
   Declare Module Export Free : STCISFREE      Ids Op       CE.Syn Syn CE.IsF.
-  Declare Module Export Wdef : STCWELLDEFINED Ids Op       CE.Syn Syn Syst Ord Var Last Def CE.IsF Free.
+  Declare Module Export Wdef : STCWELLDEFINED Ids Op       CE.Syn Syn Syst Ord Var Init Def CE.IsF Free.
   Declare Module Export SchV : STCSCHEDULINGVALIDATOR
-                                              Ids Op       CE.Syn Syn Syst Ord Var Last Def CE.IsF Free Wdef.
+                                              Ids Op       CE.Syn Syn Syst Ord Var Init Def CE.IsF Free Wdef.
   Declare Module Export Typ  : STCTYPING      Ids Op       CE.Syn Syn CE.Typ.
-  Declare Module Export Clo  : STCCLOCKING    Ids Op       CE.Syn Syn Last Var Def Syst Ord CE.Clo.
-  Declare Module Export CloSem : STCCLOCKINGSEMANTICS Ids Op OpAux CE.Syn Syn Str Last Var Def Syst Ord
+  Declare Module Export Clo  : STCCLOCKING    Ids Op       CE.Syn Syn Init Var Def Syst Ord CE.Clo.
+  Declare Module Export CloSem : STCCLOCKINGSEMANTICS Ids Op OpAux CE.Syn Syn Str Init Var Def Syst Ord
                                                      CE.Sem Sem CE.Clo Clo CE.CloSem.
 
-  Declare Module Scheduler   : STCSCHEDULE    Ids Op OpAux Str CE Syn Syst Ord Sem Typ Var Last Def Clo Free Wdef.
+  Declare Module Scheduler   : STCSCHEDULE    Ids Op OpAux Str CE Syn Syst Ord Sem Typ Var Init Def Clo Free Wdef.
 
 End STC.
 
@@ -68,17 +68,17 @@ Module StcFun
   Module Export Syst  := StcIsSystemFun    Ids Op       CE.Syn Syn.
   Module Export Ord   := StcOrderedFun     Ids Op       CE.Syn Syn Syst.
   Module Export Sem   := StcSemanticsFun   Ids Op OpAux CE.Syn Syn Syst Ord Str CE.Sem.
-  Module Export Last  := StcIsLastFun      Ids Op       CE.Syn Syn.
+  Module Export Init  := StcIsInitFun      Ids Op       CE.Syn Syn.
   Module Export Var   := StcIsVariableFun  Ids Op       CE.Syn Syn.
-  Module Export Def   := StcIsDefinedFun   Ids Op       CE.Syn Syn Var Last.
+  Module Export Def   := StcIsDefinedFun   Ids Op       CE.Syn Syn Var Init.
   Module Export Free  := StcIsFreeFun      Ids Op       CE.Syn Syn CE.IsF.
-  Module Export Wdef  := StcWellDefinedFun Ids Op       CE.Syn Syn Syst Ord Var Last Def CE.IsF Free.
+  Module Export Wdef  := StcWellDefinedFun Ids Op       CE.Syn Syn Syst Ord Var Init Def CE.IsF Free.
   Module Export SchV  := StcSchedulingValidatorFun
-                                           Ids Op       CE.Syn Syn Syst Ord Var Last Def CE.IsF Free Wdef.
+                                           Ids Op       CE.Syn Syn Syst Ord Var Init Def CE.IsF Free Wdef.
   Module Export Typ   := StcTypingFun      Ids Op       CE.Syn Syn CE.Typ.
-  Module Export Clo   := StcClockingFun    Ids Op       CE.Syn Syn Last Var Def Syst Ord CE.Clo.
-  Module Export CloSem := StcClockingSemanticsFun Ids Op OpAux CE.Syn Syn Str Last Var Def Syst Ord
+  Module Export Clo   := StcClockingFun    Ids Op       CE.Syn Syn Init Var Def Syst Ord CE.Clo.
+  Module Export CloSem := StcClockingSemanticsFun Ids Op OpAux CE.Syn Syn Str Init Var Def Syst Ord
                                                      CE.Sem Sem CE.Clo Clo CE.CloSem.
 
-  Module Scheduler    := StcScheduleFun    Ids Op OpAux Str CE Syn Syst Ord Sem Typ Var Last Def Clo Free Wdef.
+  Module Scheduler    := StcScheduleFun    Ids Op OpAux Str CE Syn Syst Ord Sem Typ Var Init Def Clo Free Wdef.
 End StcFun.
